verified/ptables.i.dfy
@@ -3,7 +3,7 @@ include "entry.s.dfy"
 
 function mkAbsPTE(pte: L2PTE): Maybe<AbsPTE>
     requires PhysBase() == KOM_DIRECTMAP_VBASE()
-    ensures var r := mkAbsPTE(pte); r.Just? ==> WellformedAbsPTE(r.v)
+    ensures WellformedAbsPTE(mkAbsPTE(pte))
 {
     match pte {
         case SecureMapping(p, w, x) => Just(
@@ -20,9 +20,18 @@ function mkAbsPTE(pte: L2PTE): Maybe<AbsPTE>
     }
 }
 
+function mkAbsL1PTE(e: Maybe<PageNr>, subpage:int): Maybe<addr>
+    requires 0 <= subpage < 4
+{
+    match e
+        case Nothing => Nothing
+        case Just(pgNr) =>
+            Just(page_paddr(pgNr) + subpage * ARM_L2PT_BYTES())
+}
+
 lemma {:axiom} lemma_l2ptesmatch(pte: L2PTE)
     requires PhysBase() == KOM_DIRECTMAP_VBASE()
-    ensures ExtractAbsL2PTE(mkL2Pte(pte)) == Just(mkAbsPTE(pte))
+    ensures ValidAbsL2PTEWord(mkL2Pte(pte)) && ExtractAbsL2PTE(mkL2Pte(pte)) == mkAbsPTE(pte)
 /* FIXME: this is really gross right now (and contains several
  * assumes!), largely due to problems in Boogie/Dafny's bitvector
  * support. It's also hopelessly unstable.
@@ -63,17 +72,12 @@ lemma {:axiom} lemma_l2ptesmatch(pte: L2PTE)
     }
 } */
 
-/*
-function getAbsPTE(d:PageDb, l2:PageNr, i:int, j:int): Maybe<AbsPTE>
-    requires validPageDb(d)
-    requires validL2PTPage(d, l2) && !hasStoppedAddrspace(d, l2)
-    requires 0 <= i < 4 && 0 <= j < ARM_L2PTES()
+lemma {:axiom} lemma_l1ptesmatch(e: Maybe<PageNr>, subpage:int)
+    requires 0 <= subpage < 4
     requires PhysBase() == KOM_DIRECTMAP_VBASE()
-    ensures var r := getAbsPTE(d, l2, i, j); r.Just? ==> WellformedAbsPTE(r.v)
-{
-    mkAbsPTE(d[l2].entry.l2pt[i * 4 + j])
-}
-*/
+    ensures ValidAbsL1PTEWord(mkL1Pte(e, subpage))
+    ensures ExtractAbsL1PTE(mkL1Pte(e, subpage)) == mkAbsL1PTE(e, subpage)
+    /* TODO: as above */
 
 function mkAbsL2PTable(e:PageDbEntryTyped, i:int): AbsL2PTable
     requires PhysBase() == KOM_DIRECTMAP_VBASE()
@@ -85,6 +89,71 @@ function mkAbsL2PTable(e:PageDbEntryTyped, i:int): AbsL2PTable
     var res := MapSeqToSeq(l2ptes, mkAbsPTE);
     assert |res| == ARM_L2PTES();
     res
+}
+
+lemma lemma_memstatecontainspage(s:memstate, p:PageNr)
+    requires SaneMem(s)
+    ensures memContainsPage(s.addresses, p)
+{
+    var va := page_monvaddr(p);
+    assert ValidMemRange(va, va + PAGESIZE());
+    reveal_ValidMemState();
+}
+
+predicate l2tablesmatch(s:memstate, p:PageNr, e:PageDbEntryTyped)
+    requires PhysBase() == KOM_DIRECTMAP_VBASE()
+    requires ValidMemState(s)
+    requires e.L2PTable? && wellFormedPageDbEntryTyped(e)
+{
+    var vbase := page_monvaddr(p);
+    ValidMemRange(vbase, vbase + PAGESIZE())
+    && forall i | 0 <= i < 4 ::
+        ValidAbsL2PTable(s, vbase + i * ARM_L2PTABLE_BYTES())
+        && ExtractAbsL2PTable(s, vbase + i * ARM_L2PTABLE_BYTES()) == mkAbsL2PTable(e, i)
+}
+
+lemma lemma_l2tablesmatch(s:memstate, p:PageNr, e:PageDbEntryTyped)
+    requires SaneMem(s)
+    requires PhysBase() == KOM_DIRECTMAP_VBASE()
+    requires e.L2PTable? && wellFormedPageDbEntryTyped(e)
+    requires pageDbL2PTableCorresponds(p, e, extractPage(s, p))
+    ensures l2tablesmatch(s, p, e)
+{
+    var l2pt := e.l2pt;
+    var base := page_monvaddr(p);
+
+    assert ARM_L2PTES() * 4 == NR_L2PTES();
+
+    forall i | 0 <= i < 4
+        ensures ValidAbsL2PTable(s, base + i * ARM_L2PTABLE_BYTES())
+        ensures ExtractAbsL2PTable(s, base + i * ARM_L2PTABLE_BYTES()) == mkAbsL2PTable(e, i) {
+
+        var subbase := base + i * ARM_L2PTABLE_BYTES();
+
+        forall j | 0 <= j < ARM_L2PTES()
+            ensures ValidAbsL2PTEWord(MemContents(s, subbase + WordsToBytes(j)))
+            ensures mkAbsPTE(l2pt[i * ARM_L2PTES() + j]) == mkAbsL2PTable(e, i)[j]
+                    == ExtractAbsL2PTE(MemContents(s, subbase + WordsToBytes(j))) {
+
+            var idx := i * ARM_L2PTES() + j;
+            var pte := l2pt[idx];
+            var a1 := base + WordsToBytes(i * ARM_L2PTES() + j);
+            var a2 := subbase + WordsToBytes(j);
+            assert a1 == a2;
+            var w := MemContents(s, a2);
+
+            assert ValidAbsL2PTEWord(w) && ExtractAbsL2PTE(w) == mkAbsPTE(pte) by {
+                lemma_memstatecontainspage(s, p);
+                reveal_pageDbL2PTableCorresponds();
+                assert w == mkL2Pte(pte);
+                assert i * ARM_L2PTABLE_BYTES() + WordsToBytes(j) == WordsToBytes(idx);
+                lemma_l2ptesmatch(pte);
+            }
+        }
+
+        assert ValidAbsL2PTable(s, subbase);
+        assert |mkAbsL2PTable(e, i)| == |ExtractAbsL2PTable(s, subbase)| == ARM_L2PTES();
+    }
 }
 
 function mkAbsPTable'(d:PageDb, l1:PageNr, idx:int): AbsPTable
@@ -113,80 +182,6 @@ function mkAbsPTable'(d:PageDb, l1:PageNr, idx:int): AbsPTable
         first + mkAbsPTable'(d, l1, idx + 1)
 }
 
-lemma lemma_memstatecontainspage(s:memstate, p:PageNr)
-    requires SaneMem(s)
-    ensures memContainsPage(s.addresses, p)
-{
-    var va := page_monvaddr(p);
-    assert ValidMemRange(va, va + PAGESIZE());
-    reveal_ValidMemState();
-}
-
-predicate l2tablesmatch(s:memstate, p:PageNr, e:PageDbEntryTyped)
-    requires PhysBase() == KOM_DIRECTMAP_VBASE()
-    requires ValidMemState(s)
-    requires e.L2PTable? && wellFormedPageDbEntryTyped(e)
-{
-    var vbase := page_monvaddr(p);
-    ValidMemRange(vbase, vbase + PAGESIZE())
-    && forall i | 0 <= i < 4 :: ExtractAbsL2PTable(s, vbase + i * ARM_L2PTABLE_BYTES(), 0)
-        == Just(mkAbsL2PTable(e, i))
-}
-
-lemma lemma_ExtractAbsL2PTable(m:memstate, vbase:addr, i:nat)
-    requires ValidMemState(m)
-    requires WordAligned(vbase)
-        && ValidMemRange(vbase, vbase + ARM_L2PTABLE_BYTES())
-    requires 0 <= i <= ARM_L2PTES()
-    requires forall j | 0 <= j < ARM_L2PTES() :: ExtractAbsL2PTE(MemContents(m, vbase + WordsToBytes(j))).Just?
-    ensures ExtractAbsL2PTable(m, vbase, i).Just?
-    ensures forall j | 0 <= j < ARM_L2PTES() - i :: ExtractAbsL2PTable(m, vbase, i).v[j] == ExtractAbsL2PTE(MemContents(m, vbase + WordsToBytes(j+i))).v
-    decreases ARM_L2PTES() - i
-{
-    if (i != ARM_L2PTES()) {
-        var r := ExtractAbsL2PTable(m, vbase, i);
-        var rest := ExtractAbsL2PTable(m, vbase, i + 1);
-        var pte := ExtractAbsL2PTE(MemContents(m, vbase + WordsToBytes(i)));
-        assert pte.Just?;
-        lemma_ExtractAbsL2PTable(m, vbase, i + 1);
-        assert rest.Just?;
-        assert r == Just([fromJust(pte)] + fromJust(rest));
-    }
-}
-
-lemma lemma_l2tablesmatch(s:memstate, p:PageNr, e:PageDbEntryTyped)
-    requires SaneMem(s)
-    requires PhysBase() == KOM_DIRECTMAP_VBASE()
-    requires e.L2PTable? && wellFormedPageDbEntryTyped(e)
-    requires pageDbL2PTableCorresponds(p, e, extractPage(s, p))
-    ensures l2tablesmatch(s, p, e)
-{
-    var l2pt := e.l2pt;
-    var base := page_monvaddr(p);
-
-    assert ARM_L2PTES() * 4 == NR_L2PTES();
-    forall i, j | 0 <= i < 4 && 0 <= j < ARM_L2PTES()
-        ensures ExtractAbsL2PTE(MemContents(s, base + WordsToBytes(i * ARM_L2PTES() + j))) == Just(mkAbsPTE(l2pt[i * ARM_L2PTES() + j])) {
-        var idx := i * ARM_L2PTES() + j;
-        var pte := l2pt[idx];
-        lemma_memstatecontainspage(s, p);
-        reveal_pageDbL2PTableCorresponds();
-        assert MemContents(s, base + WordsToBytes(idx)) == mkL2Pte(pte);
-        assert i * ARM_L2PTABLE_BYTES() + WordsToBytes(j) == WordsToBytes(idx);
-        lemma_l2ptesmatch(pte);
-    }
-
-    forall i | 0 <= i < 4
-        ensures ExtractAbsL2PTable(s, base + i * ARM_L2PTABLE_BYTES(), 0)
-        == Just(mkAbsL2PTable(e, i)) {
-        assert forall j | 0 <= j < ARM_L2PTES() ::
-            mkAbsL2PTable(e, i)[j] == mkAbsPTE(l2pt[i * ARM_L2PTES() + j]) == ExtractAbsL2PTE(MemContents(s, base + i * ARM_L2PTABLE_BYTES() + WordsToBytes(j))).v;
-        lemma_ExtractAbsL2PTable(s, base + i * ARM_L2PTABLE_BYTES(), 0);
-        assert |mkAbsL2PTable(e, i)| == |ExtractAbsL2PTable(s, base + i * ARM_L2PTABLE_BYTES(), 0).v| == ARM_L2PTES();
-        assert forall j | 0 <= j < ARM_L2PTES() :: base + i * ARM_L2PTABLE_BYTES() + WordsToBytes(j) == base + WordsToBytes(j + i*ARM_L2PTES());
-    }
-}
-
 function mkAbsPTable(d:PageDb, l1:PageNr): AbsPTable
     requires PhysBase() == KOM_DIRECTMAP_VBASE()
     requires validPageDb(d)
@@ -202,9 +197,48 @@ lemma lemma_ptablesmatch(s:memstate, d:PageDb, l1p:PageNr)
     requires validPageDb(d)
     requires nonStoppedL1(d, l1p)
     requires pageDbCorresponds(s, d)
-    ensures ExtractAbsL1PTable(s, page_monvaddr(l1p), 0) == Just(mkAbsPTable(d, l1p))
+    ensures ValidAbsL1PTable(s, page_monvaddr(l1p))
+    ensures ExtractAbsL1PTable(s, page_monvaddr(l1p)) == mkAbsPTable(d, l1p)
 {
-    assume false; // TODO
+    var l1pt := d[l1p].entry.l1pt;
+    var l1base := page_monvaddr(l1p);
+
+    assert validL1PTable(d, l1p) by {reveal_validPageDb();}
+    lemma_memstatecontainspage(s, l1p);
+
+    assert pageDbL1PTableCorresponds(l1p, d[l1p].entry, extractPage(s, l1p)) by { reveal_pageContentsCorresponds(); }
+    reveal_pageDbL1PTableCorresponds();
+
+    assert ARM_L1PTES() == 4 * NR_L1PTES();
+
+    forall i, j | 0 <= i < NR_L1PTES() && 0 <= j < 4
+        ensures ValidAbsL1PTEWord(MemContents(s, l1base + WordsToBytes(i * 4 + j)))
+        ensures ExtractAbsL1PTE(MemContents(s, l1base + WordsToBytes(i * 4 + j))) == mkAbsL1PTE(l1pt[i], j) {
+        var ptew := MemContents(s, l1pteoffset(l1base, i, j));
+        lemma_l1ptesmatch(l1pt[i], j);
+    }
+
+    forall i | 0 <= i < NR_L1PTES()
+        ensures l1pt[i].Just? ==> l2tablesmatch(s, l1pt[i].v, d[l1pt[i].v].entry)
+    {
+        var l1e := l1pt[i];
+        if l1e.Just? {
+            var l2p := l1e.v;
+            assert validL1PTE(d, l2p);
+            assert pageDbL2PTableCorresponds(l2p, d[l2p].entry, extractPage(s, l2p)) by { reveal_pageContentsCorresponds(); }
+            lemma_l2tablesmatch(s, l2p, d[l2p].entry);
+        }
+    }
+
+    assume false; // TODO!
+
+    assert 4 * ARM_L2PT_BYTES() == PAGESIZE();
+
+    assert forall i | 0 <= i < NR_L1PTES() && l1pt[i].Just?
+        :: page_paddr(l1pt[i].v) < SecurePhysBase() + KOM_SECURE_RESERVE();
+
+    assert forall i, j | 0 <= i < NR_L1PTES() && 0 <= j < 4 && l1pt[i].Just?
+        :: ValidAbsL2PTable(s, mkAbsL1PTE(l1pt[i], j).v + PhysBase());
 }
 
 lemma UserExecutionMemInvariant(s:state, s':state, d:PageDb, l1:PageNr)
@@ -216,11 +250,6 @@ lemma UserExecutionMemInvariant(s:state, s':state, d:PageDb, l1:PageNr)
     requires s.conf.ttbr0.ptbase == page_paddr(l1)
     ensures WSMemInvariantExceptAddrspaceAtPage(s, s', d, l1)
 {
-    var l1pg := extractPage(s.m, l1);
-    var e := d[l1].entry;
-    assert e.L1PTable? && wellFormedPageDbEntryTyped(e);
-    assert pageContentsCorresponds(l1, d[l1], l1pg);
-    reveal_pageContentsCorresponds();
-    assert pageDbL1PTableCorresponds(l1, e, l1pg);
+    lemma_ptablesmatch(s.m, d, l1);
     assume false; // TODO
 }
